reworked fixpoint through tactics (see MPLSVectorizedProof for an example of usage)

lib/Benchmarks/MPLSVectorizedProof.v
@@ -9,36 +9,20 @@ Notation conf := (P4automaton.configuration (P4A.interp A)).
 Notation start_left :=  Plain.ParseMPLS.
 Notation start_right := Unrolled.ParseMPLS.
 
-Fixpoint reachable_states_len' (r: Reachability.state_pairs A) (fuel: nat) :=
-  match fuel with
-  | 0 => None
-  | S x =>
-    let nxt := Reachability.reachable_step r in
-    let nxt_len := length nxt in
-    if Nat.eq_dec (length nxt) (length r) then Some nxt_len
-    else
-      reachable_states_len' nxt x
-  end.
+(* Eval vm_compute in (length (Reachability.valid_state_templates A)). *)
 
-Definition r_depth : nat.
-refine (
-let s := ({| st_state := inl (inl start_left); st_buf_len := 0 |},
-          {| st_state := inl (inr start_right); st_buf_len := 0 |}) in
-let r := reachable_states_len' [s] 1000 in
-_).
-vm_compute in r.
-match goal with
-| _ := Some ?x |- _ => exact x
-end.
-Defined.
+Definition r_states : Reachability.state_pairs A.
+  evar (r: Reachability.state_pairs A).
+  assert (Reachability.reachable_states_wit _ start_left start_right r).
 
 
-Definition r_states :=
-  Eval vm_compute in (Reachability.reachable_states
+
+Definition r_states := (Reachability.reachable_states
                         A
-                        r_depth
                         start_left
                         start_right).
+
+                
 
 Definition top : Relations.rel conf := fun _ _ => True.
 Definition top' : Relations.rel (state_template A) := fun _ _ => True.
@@ -89,12 +73,12 @@ Lemma prebisim_mpls_unroll:
                     (wp r_states)
                     top
                     []
-                    (mk_init _ _ _ _ A r_depth start_left start_right)
+                    (mk_init _ _ _ A r_depth start_left start_right)
                     q1 q2.
 Proof.
   intros.
 
-  set (rel0 := (mk_init _ _ _ _ _ _ _ _)).
+  set (rel0 := (mk_init _ _ _ _ _ _ _)).
   vm_compute in rel0.
   subst rel0.
 
