lib/Utils/FunctionalFP.v
@@ -1,5 +1,5 @@
 
-Section FunctionalFP.
+Section FuelFP.
   Variable (A: Type).
   Variable (f: A -> A).
 
@@ -19,7 +19,7 @@ Section FunctionalFP.
       if eqb nxt a then nxt else f (iter' n' a)
     end.
 
-  Variable (eqb_sound: forall a a', eqb a a' = true <-> a = a').
+  Variable (eqb_sound: forall x, eqb (f x) x = true <-> (f x) = x).
 
   Lemma iter_iter' : 
     forall n a,
@@ -30,7 +30,7 @@ Section FunctionalFP.
     - simpl. reflexivity.
     - unfold iter; fold iter.
       unfold iter'; fold iter'.
-      pose proof (@eqb_sound (f a) a).
+      pose proof (@eqb_sound a).
       destruct (eqb _ _) eqn:?.
       + destruct H as [H' _].
         erewrite H'; trivial.
@@ -38,11 +38,69 @@ Section FunctionalFP.
 
         destruct n; simpl iter'; [eapply H'; trivial|].
 
-        specialize (@eqb_sound (f a) a).
+        specialize (@eqb_sound a).
         destruct eqb_sound as [_ H''].
         erewrite H''; erewrite H'; trivial.
         eapply H'; trivial.
       + erewrite IHn; trivial.
   Qed.
 
-End FunctionalFP.
+End FuelFP.
+
+
+Section ExactFP.
+  Variable (A: Type).
+  Variable (f: A -> A).
+
+  Definition fp := {x | f x = x}.
+
+  Inductive fp_wit : A -> A -> Type := 
+  | FPDone : forall x, 
+    f x = x -> fp_wit x x
+  | FPIter : forall x y,
+    fp_wit (f x) y -> fp_wit x y.
+
+  (* extract the final fp out from a construction of its fp-ness *)
+  Fixpoint wit_conv {x y} (wit: fp_wit x y) : fp := 
+    match wit with 
+    | FPDone _ pf => exist _ _ pf
+    | FPIter _ _ wit' => wit_conv wit'
+    end.
+  
+End ExactFP.
+
+Ltac solve_fp_wit := 
+  repeat (
+    match goal with 
+    | |- fp_wit _ _ _ _ => 
+      eapply FPDone;
+      simpl;
+      trivial
+    | |- fp_wit _ _ ?X _ => 
+      econstructor;
+      set (foo := X);
+      vm_compute in foo;
+      subst foo
+    end
+  ).
+
+Definition collatz (n: nat) := 
+  match n with
+  | 1 => 1
+  | n => 
+    if Nat.even n then Nat.div n 2 else 3 * n + 1
+  end.
+
+Definition collatz_10 : fp _ collatz.
+  evar (n: nat).
+  assert (fp_wit _ collatz 10 n).
+  solve_fp_wit.
+  subst n.
+  eapply FPDone.
+  compute.
+  trivial.
+  subst n.
+  simpl collatz in X.
+  eapply wit_conv.
+  exact X.
+Defined.
